Allow left-hand sides of a let expression to be patterns (like in the case of a match expression). Moved the implementation of CondApplyBox, BoxIfNecessary, CondApplyUnbox, and ModeledAsBoxType from class ExpressionTranslator to class Translator. Fixed compilation of match expressions, to allow them anywhere.

Binaries/DafnyRuntime.cs
@@ -627,5 +627,6 @@ namespace Dafny
     {
       return u;
     }
+    public delegate Result Function<Input,Result>(Input input);
   }
 }
